Use a stronger induction principle for ChainTrace
Since we will need to reason over specific inhabitants of traces, this
is required to prove many interesting properties by induction, as
explained to me by Danil Annenkov.

src/Blockchain.v
@@ -700,6 +700,7 @@ Definition empty_env : Environment :=
 (* The ChainTrace captures that there is a valid execution where,
 starting from one environment and queue of actions, we end up in a
 different environment and queue of actions. *)
+Unset Elimination Schemes.
 Inductive ChainTrace :
   Environment -> list Action ->
   Environment -> list Action -> Prop :=
@@ -744,12 +745,23 @@ Inductive ChainTrace :
         Permutation to_queue to_queue' ->
         ChainTrace from from_queue to to_queue'.
 
+(* The normal induction principle generated for propositions does not
+allow the picked proposition to depend on the inhabitant of the
+proposition. However, for our traces, we will often want to prove
+properties that rely on the specific inhabitant. For instance when we
+need to reason about prefixes or suffixes. Thus we derive a normal
+principle instead. As an example, rhis is necessary for the proofs
+about trace_app below. This difference between inductives in Prop and
+Type, and the solution was highlighted to me by Danil Annenkov. *)
+Scheme ChainTrace_ind := Induction for ChainTrace Sort Prop.
+Set Elimination Schemes.
+
 Fixpoint trace_app
-           {from mid to : Environment}
-           {from_queue mid_queue to_queue : list Action}
-           (c1 : ChainTrace from from_queue mid mid_queue)
-           (c2 : ChainTrace mid mid_queue to to_queue)
-  : ChainTrace from from_queue to to_queue :=
+            {from mid to : Environment}
+            {from_queue mid_queue to_queue : list Action}
+            (c1 : ChainTrace from from_queue mid mid_queue)
+            (c2 : ChainTrace mid mid_queue to to_queue)
+   : ChainTrace from from_queue to to_queue :=
   match c2 with
   | ctrace_refl => fun c1 => c1
   | ctrace_block pref valid from_accs eq =>
@@ -783,27 +795,28 @@ Infix "`prefix_of`" := trace_prefix (at level 70) : trace_scope.
 Infix "`suffix_of`" := trace_suffix (at level 70) : trace_scope.
 
 Section Theories.
-Fixpoint trace_app_refl_l
+Lemma trace_app_refl_l
       {from to from_queue to_queue}
       (trace : ChainTrace from from_queue to to_queue) :
   ctrace_refl ++ trace = trace.
 Proof.
-  destruct trace; try reflexivity; cbn;
+  induction trace; cbn; auto;
     match goal with
-    | [|- context[ctrace_refl ++ ?a]] => now rewrite (trace_app_refl_l _ _ _ _ a)
+    | [IH: _ |- _] => now rewrite IH
     end.
 Qed.
 
-Fixpoint trace_app_assoc
+Lemma trace_app_assoc
       {env1 env2 env3 env4 queue1 queue2 queue3 queue4}
       (c1 : ChainTrace env1 queue1 env2 queue2)
       (c2 : ChainTrace env2 queue2 env3 queue3)
       (c3 : ChainTrace env3 queue3 env4 queue4) :
   c1 ++ c2 ++ c3 = (c1 ++ c2) ++ c3.
 Proof.
-  destruct c3; try reflexivity; cbn;
+  revert env1 env2 queue1 queue2 c1 c2.
+  induction c3; intros env1 env2 queue1 queue2 c1 c2; cbn; auto;
     match goal with
-    | [|- context[?a ++ ?b ++ ?c]] => now rewrite (trace_app_assoc _ _ _ _ _ _ _ _ a b c)
+    | [IH: _ |- _] => now rewrite IH
     end.
 Qed.
 End Theories.
